reflex case stadies/Fridge/Fridge_VC747.thy
@@ -1,0 +1,19 @@
+theory Fridge_VC747
+imports FridgeTheory
+begin
+
+lemma
+ assumes base_inv:"(inv st0)"
+ and st1:"(st1=(setVarBool st0 ''inp_3'' inp_3))"
+ and st2:"(st2=(setVarBool st1 ''inp_2'' inp_2))"
+ and st3:"(st3=(setVarBool st2 ''inp_1'' inp_1))"
+ and st4:"(st4=(setVarBool st3 ''inp_5'' inp_5))"
+ and st5:"(st5=(setVarBool st4 ''inp_4'' inp_4))"
+ and st5_Init_state:"(getPstate st5 ''Init'')=''error''"
+ and st5_FridgrDoorController_state:"(getPstate st5 ''FridgrDoorController'')=''error''"
+ and st5_FridgeCompressorController_state:"(getPstate st5 ''FridgeCompressorController'')=''error''"
+ and st5_FreezerCompressorController_state:"(getPstate st5 ''FreezerCompressorController'')=''error''"
+ and st6:"(st6=(toEnv st5))"
+shows "(inv st6)"
+
+end
