reflex case stadies/HandDryer/HandDryer_VC3.thy
@@ -50,11 +50,11 @@ next
     show "R1_sub1 st3"
     proof(simp add: R1_sub1_def; intro allI; rule impI)
       fix s1 s2
-      assume prems:"R1_sub1_prems st3 s1 s2"
+      assume prems:"R1_sub2_prems st3 s1 s2"
       thus "R1_sub2 st3 s2"
-      proof (simp only: R1_sub1_prems_def; cases)
+      proof (simp only: R1_sub2_prems_def; cases)
         assume 1:"s2=st3"
-        have "R1_sub2_prems st3 s2 s2 \<and> R1_sub3 s2 s2"
+        have "R1_sub3_prems st3 s2 s2 \<and> R1_sub3 s2 s2"
         proof 
           have 2:"toEnvP s2 \<and>substate s2 s2 \<and>substate s2 st3" using 1 st3 by (simp)
           have 3:"toEnvNum s2 s2 \<le> 1" using toEnvNum_id by simp
@@ -66,17 +66,17 @@ next
             then have "getVarBool st3 ''out_1'' = True" using 1 5 ex extraInv_def assms by blast
             thus "getVarBool s2 ''out_1'' = True" using 1 by simp
           qed
-          thus "R1_sub2_prems st3 s2 s2" using 1 2 3 4 R1_sub2_prems_def by auto
+          thus "R1_sub3_prems st3 s2 s2" using 1 2 3 4 R1_sub3_prems_def by auto
         next
-          show "R1_sub3 s2 s2" using 1 assms R1_sub3_def substate_asym by blast
+          show "R1_sub3 s2 s2" using 1 assms R1_sub3_def R1_sub4_prems_def substate_asym by blast
         qed
         thus ?thesis using R1_sub2_def by blast
       next
         assume 1: "s2\<noteq>st3"
-        then have "substate s2 st0" using prems assms R1_sub1_prems_def by (simp split: if_splits)
-        then obtain "R1_sub2 st0 s2" using assms prems inv1_def R1_def R1_sub1_def R1_sub1_prems_def by auto
-        then obtain s4 where 3:"R1_sub2_prems st0 s2 s4 \<and> R1_sub3 s2 s4" using R1_sub2_def by auto
-        thus ?thesis using 3 assms R1_sub2_def R1_sub2_prems_def substate.simps by metis
+        then have "substate s2 st0" using prems assms R1_sub2_prems_def by (simp split: if_splits)
+        then obtain "R1_sub2 st0 s2" using assms prems inv1_def R1_def R1_sub1_def R1_sub2_prems_def by auto
+        then obtain s4 where 3:"R1_sub3_prems st0 s2 s4 \<and> R1_sub3 s2 s4" using R1_sub2_def by auto
+        thus ?thesis using 3 assms R1_sub2_def R1_sub3_prems_def substate.simps by metis
       qed
     qed
   qed
@@ -100,14 +100,14 @@ next
     show "R2_sub1 st3"
     proof (simp only:R2_sub1_def; rule allI;rule allI;rule impI)
       fix s1 s2
-      assume prems:"R2_sub1_prems st3 s1 s2"
+      assume prems:"R2_sub2_prems st3 s1 s2"
       thus "getVarBool s2 ''out_1'' = False"
-      proof (simp only: R2_sub1_prems_def; cases)
+      proof (simp only: R2_sub2_prems_def; cases)
         assume 1: "s2=st3"
-        thus ?thesis using assms prems R2_sub1_prems_def by auto
+        thus ?thesis using assms prems R2_sub2_prems_def by auto
       next
         assume 2: "s2\<noteq>st3"
-        thus ?thesis using assms prems R2_def R2_sub1_def R2_sub1_prems_def inv2_def 
+        thus ?thesis using assms prems R2_def R2_sub1_def R2_sub2_prems_def inv2_def 
         by (metis (no_types, lifting) state.distinct(25) substate.simps(2) substate.simps(3) substate.simps(8) toEnvP.elims(2)) 
       qed
     qed
@@ -132,21 +132,21 @@ next
     show "R3_sub1 st3"
     proof(simp only: R3_sub1_def; intro allI; rule impI)
       fix s1 s2
-      assume prems:"R3_sub1_prems st3 s1 s2" 
-      then obtain "20 \<le> toEnvNum s2 st3" using R3_sub1_prems_def by auto
+      assume prems:"R3_sub2_prems st3 s1 s2" 
+      then obtain "20 \<le> toEnvNum s2 st3" using R3_sub2_prems_def by auto
       from le_imp_less_or_eq[OF this] show "R3_sub2 st3 s2"
         apply (rule disjE)
       proof -
         assume 1:"20 < toEnvNum s2 st3"
-        have 2: "substate s2 st0" using assms prems R3_sub1_prems_def substate_eq_or_predEnv toEnvNum_id by (simp split:if_splits)
+        have 2: "substate s2 st0" using assms prems R3_sub2_prems_def substate_eq_or_predEnv toEnvNum_id by (simp split:if_splits)
         obtain "R3_sub1 st0" using prems R3_def base_inv inv3_def by auto
-        then have "R3_sub2 st0 s2" using 1 2 prems assms R3_sub2_def R3_sub1_prems_def R3_sub1_def by (auto simp add: split:if_splits)
-        then obtain s4 where 3: "R3_sub2_prems st0 s2 s4 \<and> R3_sub3 s2 s4" using R3_sub2_def by auto
-        then have "R3_sub2_prems st3 s2 s4 \<and> R3_sub3 s2 s4" using assms R3_sub2_prems_def by auto
+        then have "R3_sub2 st0 s2" using 1 2 prems assms R3_sub2_def R3_sub2_prems_def R3_sub1_def by (auto simp add: split:if_splits)
+        then obtain s4 where 3: "R3_sub3_prems st0 s2 s4 \<and> R3_sub3 s2 s4" using R3_sub2_def by auto
+        then have "R3_sub3_prems st3 s2 s4 \<and> R3_sub3 s2 s4" using assms R3_sub3_prems_def by auto
         thus ?thesis using R3_sub2_def by auto
       next
         assume 1: "20 = toEnvNum s2 st3"
-        have 2:"R3_sub3 s2 s2" using substate_asym R3_sub3_def by auto
+        have 2:"R3_sub3 s2 s2" using substate_asym R3_sub3_def R3_sub4_prems_def by auto
         show ?thesis
         proof -
           define s5::state where "s5=s2"
@@ -154,7 +154,7 @@ next
                 \<longrightarrow> pred3 st3 s2 s5" including pred3_defs
              proof(induction rule: state_down_ind)
                case 1
-               then show ?case using prems assms R3_sub1_prems_def by auto
+               then show ?case using prems assms R3_sub2_prems_def by auto
              next
                case 2
                then show ?case
@@ -182,7 +182,7 @@ next
                    assume 6: "getVarBool (predEnv s5) ''out_1'' = False \<or>
                               getVarBool (predEnv s5) ''inp_1'' = True"
                    have 7: "substate (predEnv s5) st3" using predEnv_substate substate_trans 3 by blast
-                   have 8: "substate s2 (predEnv s5)" using 3(2) substate_eq_or_predEnv prems R3_sub1_prems_def by auto
+                   have 8: "substate s2 (predEnv s5)" using 3(2) substate_eq_or_predEnv prems R3_sub2_prems_def by auto
                    have "pred3_sub2_prems st3 s2 (predEnv s5) (predEnv s5) \<and> pred3_sub3 (predEnv s5) (predEnv s5)"
                    proof -
                      have "toEnvP (predEnv s5)" using predEnvP_or_emptyState[of s5] 
@@ -191,7 +191,7 @@ next
                        thus ?thesis by assumption
                      next 
                        assume "predEnv s5 = emptyState"
-                       thus ?thesis using 8 prems R3_sub1_prems_def by (metis substate.simps(1))
+                       thus ?thesis using 8 prems R3_sub2_prems_def by (metis substate.simps(1))
                      qed
                      moreover have "substate (predEnv s5) (predEnv s5)" using substate_refl by auto
                      moreover have "substate (predEnv s5) st3" using 7 by assumption
@@ -225,7 +225,7 @@ next
                  qed
                qed
              qed
-             thus ?thesis using 2 s5_def R3_sub2_def R3_sub2_prems_def R3_sub3_def substate_refl prems R3_sub1_prems_def including pred3_defs by auto
+             thus ?thesis using 2 s5_def R3_sub2_def R3_sub3_prems_def R3_sub3_def substate_refl prems R3_sub2_prems_def including pred3_defs by auto
            qed
          qed
        qed
@@ -251,22 +251,16 @@ next
     proof (simp only:R4_sub1_def;intro allI; rule impI)
       fix s1 s2
       assume prems: 
-        "substate s1 s2 \<and>
-        substate s2 st3 \<and> 
-        toEnvP s1 \<and> 
-        toEnvP s2 \<and>
-        toEnvNum s1 s2 = 1 \<and> 
-        getVarBool s1 ''out_1'' = True \<and>
-        getVarBool s2 ''inp_1'' = True"
+        "R4_sub2_prems st3 s1 s2"
       thus "getVarBool s2 ''out_1'' = True"
       proof (cases)
         assume 1:"s2=st3"
-        thus ?thesis using assms prems 
+        thus ?thesis using assms prems R4_sub2_prems_def
         by (metis R4_def add_cancel_right_left getVarBool.simps(2) getVarBool.simps(3) getVarBool.simps(8) inv4_def substate.simps(2) substate.simps(3) substate.simps(8) substate_toEnvNum_id toEnvNum.simps(2) toEnvNum.simps(3) toEnvNum.simps(8))
       next
         assume 1: "s2\<noteq>st3"
-        then have 2: "substate s2 st0" using prems assms R1_sub1_prems_def by (simp split: if_splits)
-        thus ?thesis using R4_def R4_sub1_def base_inv inv4_def prems by blast
+        then have 2: "substate s2 st0" using prems assms R4_sub2_prems_def by (simp split: if_splits)
+        thus ?thesis using R4_def R4_sub1_def R4_sub2_prems_def base_inv inv4_def prems by metis
       qed
     qed
   qed
