reflex case stadies/HandDryer/HandDryer_VC4.thy
@@ -35,24 +35,24 @@ next
     show "R1_sub1 st4"
     proof (simp add:R1_sub1_def; intro allI;rule impI)
       fix s1 s2
-      assume prems:"R1_sub1_prems st4 s1 s2"
+      assume prems:"R1_sub2_prems st4 s1 s2"
       thus "R1_sub2 st4 s2"
-      proof (simp only: R1_sub1_prems_def; cases)
+      proof (simp only: R1_sub2_prems_def; cases)
         assume 1:"s2=st4"
-        have "R1_sub2_prems st4 s2 s2 \<and> R1_sub3 s2 s2"
+        have "R1_sub3_prems st4 s2 s2 \<and> R1_sub3 s2 s2"
         proof
-          show "R1_sub2_prems st4 s2 s2" using 1 assms R1_sub2_prems_def R1_sub1_prems_def prems by auto
+          show "R1_sub3_prems st4 s2 s2" using 1 assms R1_sub3_prems_def R1_sub2_prems_def prems by auto
         next
-          show "R1_sub3 s2 s2" using 1 assms R1_sub3_def substate_asym by blast
+          show "R1_sub3 s2 s2" using 1 assms R1_sub3_def R1_sub4_prems_def substate_asym by blast
         qed
         thus ?thesis using R1_sub2_def by blast
       next
         assume 2:"s2\<noteq>st4"
-        then have "substate s2 st0" using prems assms R1_sub1_prems_def substate.simps
+        then have "substate s2 st0" using prems assms R1_sub2_prems_def substate.simps
         by (metis toEnvP.simps(3) toEnvP.simps(7))
-        then obtain "R1_sub2 st0 s2" using assms prems inv1_def R1_def R1_sub1_def R1_sub1_prems_def by meson
-        then obtain s4 where "R1_sub2_prems st0 s2 s4 \<and> R1_sub3 s2 s4" using R1_sub2_def by auto
-        thus ?thesis using assms R1_sub2_def R1_sub2_prems_def substate.simps by metis
+        then obtain "R1_sub2 st0 s2" using assms prems inv1_def R1_def R1_sub1_def R1_sub2_prems_def by meson
+        then obtain s4 where "R1_sub3_prems st0 s2 s4 \<and> R1_sub3 s2 s4" using R1_sub2_def by auto
+        thus ?thesis using assms R1_sub2_def R1_sub3_prems_def substate.simps by metis
       qed
     qed
   qed
@@ -70,7 +70,7 @@ lemma
 shows "(inv2 st4)"
 proof -
   from assms show ?thesis
-  apply (simp only: inv2_def assms R2_def R2_sub1_def R2_sub1_prems_def)
+  apply (simp only: inv2_def assms R2_def R2_sub1_def R2_sub2_prems_def)
     apply (intro conjI)
       apply auto
     using extra assms by presburger
@@ -96,21 +96,21 @@ next
     show "R3_sub1 st4"
     proof(simp only: R3_sub1_def; intro allI; rule impI)
       fix s1 s2
-      assume prems:"R3_sub1_prems st4 s1 s2" 
-      then obtain "20 \<le> toEnvNum s2 st4" using R3_sub1_prems_def by auto
+      assume prems:"R3_sub2_prems st4 s1 s2" 
+      then obtain "20 \<le> toEnvNum s2 st4" using R3_sub2_prems_def by auto
       from le_imp_less_or_eq[OF this] show "R3_sub2 st4 s2"
         apply (rule disjE)
       proof -
         assume 1:"20 < toEnvNum s2 st4"
-        have 2: "substate s2 st0" using assms prems R3_sub1_prems_def substate_eq_or_predEnv toEnvNum_id by (simp split:if_splits)
+        have 2: "substate s2 st0" using assms prems R3_sub2_prems_def substate_eq_or_predEnv toEnvNum_id by (simp split:if_splits)
         obtain "R3_sub1 st0" using prems R3_def base_inv inv3_def by auto
-        then have "R3_sub2 st0 s2" using 1 2 prems assms R3_sub2_def R3_sub1_prems_def R3_sub1_def by (auto simp add: split:if_splits)
-        then obtain s4 where 3: "R3_sub2_prems st0 s2 s4 \<and> R3_sub3 s2 s4" using R3_sub2_def by auto
-        then have "R3_sub2_prems st4 s2 s4 \<and> R3_sub3 s2 s4" using assms R3_sub2_prems_def by auto
+        then have "R3_sub2 st0 s2" using 1 2 prems assms R3_sub2_def R3_sub2_prems_def R3_sub1_def by (auto simp add: split:if_splits)
+        then obtain s4 where 3: "R3_sub3_prems st0 s2 s4 \<and> R3_sub3 s2 s4" using R3_sub2_def by auto
+        then have "R3_sub3_prems st4 s2 s4 \<and> R3_sub3 s2 s4" using assms R3_sub3_prems_def by auto
         thus ?thesis using R3_sub2_def by auto
       next
         assume 1: "20 = toEnvNum s2 st4"
-        have 2:"R3_sub3 s2 s2" using substate_asym R3_sub3_def by auto
+        have 2:"R3_sub3 s2 s2" using substate_asym R3_sub3_def R3_sub4_prems_def by auto
         show ?thesis
         proof -
           define s5::state where "s5=s2"
@@ -118,7 +118,7 @@ next
                 \<longrightarrow> pred3 st4 s2 s5" including pred3_defs
              proof(induction rule: state_down_ind)
                case 1
-               then show ?case using prems assms R3_sub1_prems_def by auto
+               then show ?case using prems assms R3_sub2_prems_def by auto
              next
                case 2
                then show ?case
@@ -146,7 +146,7 @@ next
                    assume 6: "getVarBool (predEnv s5) ''out_1'' = False \<or>
                               getVarBool (predEnv s5) ''inp_1'' = True"
                    have 7: "substate (predEnv s5) st4" using predEnv_substate substate_trans 3 by blast
-                   have 8: "substate s2 (predEnv s5)" using 3(2) substate_eq_or_predEnv prems R3_sub1_prems_def by auto
+                   have 8: "substate s2 (predEnv s5)" using 3(2) substate_eq_or_predEnv prems R3_sub2_prems_def by auto
                    have "pred3_sub2_prems st4 s2 (predEnv s5) (predEnv s5) \<and> pred3_sub3 (predEnv s5) (predEnv s5)"
                    proof -
                      have "toEnvP (predEnv s5)" using predEnvP_or_emptyState[of s5] 
@@ -155,7 +155,7 @@ next
                        thus ?thesis by assumption
                      next 
                        assume "predEnv s5 = emptyState"
-                       thus ?thesis using 8 prems R3_sub1_prems_def by (metis substate.simps(1))
+                       thus ?thesis using 8 prems R3_sub2_prems_def by (metis substate.simps(1))
                      qed
                      moreover have "substate (predEnv s5) (predEnv s5)" using substate_refl by auto
                      moreover have "substate (predEnv s5) st4" using 7 by assumption
@@ -189,7 +189,7 @@ next
                  qed
                qed
              qed
-             thus ?thesis using 2 s5_def R3_sub2_def R3_sub2_prems_def R3_sub3_def substate_refl prems R3_sub1_prems_def including pred3_defs by auto
+             thus ?thesis using 2 s5_def R3_sub2_def R3_sub3_prems_def R3_sub3_def substate_refl prems R3_sub2_prems_def including pred3_defs by auto
            qed
          qed
        qed
@@ -217,21 +217,15 @@ next
     proof (simp only:R4_sub1_def;intro allI; rule impI)
       fix s1 s2
       assume prems: 
-        "substate s1 s2 \<and>
-        substate s2 st4 \<and> 
-        toEnvP s1 \<and> 
-        toEnvP s2 \<and>
-        toEnvNum s1 s2 = 1 \<and> 
-        getVarBool s1 ''out_1'' = True \<and>
-        getVarBool s2 ''inp_1'' = True"
+        "R4_sub2_prems st4 s1 s2"
       thus "getVarBool s2 ''out_1'' = True"
       proof (cases)
         assume 1:"s2=st4"
         thus ?thesis using assms prems by auto
       next
         assume 1: "s2\<noteq>st4"
-        then have 2: "substate s2 st0" using prems assms R1_sub1_prems_def by (simp split: if_splits)
-        thus ?thesis using R4_def R4_sub1_def base_inv inv4_def prems by blast
+        then have 2: "substate s2 st0" using prems assms R4_sub2_prems_def by (simp split: if_splits)
+        thus ?thesis using R4_def R4_sub1_def R4_sub2_prems_def base_inv inv4_def prems by metis
       qed
     qed
   qed
